Util.v
@@ -2,7 +2,12 @@
  *** Utility functions and lemmas
  ***)
 
-Add LoadPath "." as MetaSlang.
+Require Export String.
+Require Export List.
+Require Export Coq.Logic.FunctionalExtensionality.
+Require Export Coq.Logic.EqdepFacts.
+Require Export Coq.Logic.Eqdep_dec.
+
 
 (* helper function for eliminating ors *)
 Definition or_proj_r A B : ~A -> A \/ B -> B.
@@ -16,4 +21,66 @@ Definition or_proj_l A B : ~B -> A \/ B -> A.
   intros not_B or; destruct or.
   assumption.
   elimtype False; apply not_B; assumption.
+Qed.
+
+
+(*** UIP (and friends) for lists of strings ***)
+
+(* decidability of equality for lists of strings *)
+Module DecidableSetListString.
+  Definition U := list string.
+  Lemma eq_dec : forall x y:U, {x=y} + {x<>y}.
+    apply list_eq_dec; apply string_dec.
+  Qed.
+End DecidableSetListString.
+
+(* EqDep module for lists of strings *)
+Module EqDepListString := DecidableEqDep (DecidableSetListString).
+
+Definition UIP_flds flds1 flds2 (p1 p2 : flds1 = flds2) : p1 = p2 :=
+  EqDepListString.UIP flds1 flds2 p1 p2.
+
+Definition UIP_refl_flds flds (p : flds = flds) : p = eq_refl :=
+  EqDepListString.UIP_refl flds p.
+
+Definition eq_dep_eq_flds :
+  forall P {flds} {x y : P flds}, eq_dep _ P flds x flds y -> x = y :=
+  EqDepListString.eq_dep_eq.
+
+(* inj_pair2 for lists of strings *)
+Definition inj_pair2_flds {flds : list string} {A a b} :
+  existT A flds a = existT A flds b -> a = b :=
+  EqDepListString.inj_pairT2 A flds a b.
+
+
+(*** helpers for proving eq_dep goals ***)
+
+Lemma eq_dep_commute A B (a1 a2 : A) (b1 : B a1) (b2 : B a2)
+      C (f : forall x (y : B x), C x y) :
+  eq_dep _ _ a1 b1 a2 b2 ->
+  eq_dep _ (fun tup => C (projT1 tup) (projT2 tup))
+         (existT B a1 b1) (f a1 b1)
+         (existT B a2 b2) (f a2 b2).
+  intro e; induction e.
+  apply eq_dep_intro.
+Qed.
+
+Lemma eq_dep_ctx A B (a1 a2 : A) (b1 : B a1) (b2 : B a2)
+      A' (f : A -> A')
+      B' (g : forall x, B x -> B' (f x)) :
+  eq_dep _ _ a1 b1 a2 b2 ->
+  eq_dep _ _ (f a1) (g a1 b1) (f a2) (g a2 b2).
+  intro e; induction e.
+  apply eq_dep_intro.
+Qed.
+
+Lemma eq_dep_flds_fun U B (a1 a2 : list string)
+      (b1 : U -> B a1) (b2 : U -> B a2) (e : a1 = a2) :
+  (forall u, eq_dep _ B a1 (b1 u) a2 (b2 u)) ->
+  eq_dep _ (fun a => U -> B a) a1 b1 a2 b2.
+  revert b1 b2; rewrite e; intros.
+  rewrite (functional_extensionality_dep
+             _ _
+             (fun u' => eq_dep_eq_flds _ (H u'))).
+  apply eq_dep_intro.
 Qed.
